Project/ModelInterp.lean
@@ -1,9 +1,9 @@
 import Cslib.Languages.LambdaCalculus.LocallyNameless.Untyped.FullBeta
-import src.AndrejBauer.GraphModel
-import src.EngelerModel
-import src.ChurchRosser
-import src.LambdaTheory.Basic
-import src.LCresults
+import Project.AndrejBauer.GraphModel
+import Project.EngelerModel
+import Project.ChurchRosser
+import Project.LambdaTheory.Basic
+import Project.LCresults
 
 open F_G_equal
 open Listing
@@ -16,23 +16,27 @@ variable {Var : Type u} [DecidableEq Var] [HasFresh Var]
 variable {α : Type} [Listing α]
 
 @[simp]
-def subst_rho (ρ : ℕ → Set α) (n : ℕ) (d : Set α) : ℕ → Set α :=
+def subst_ρ (ρ : ℕ → Set α) (n : ℕ) (d : Set α) : ℕ → Set α :=
   fun x => if x = n then d else ρ (x)
 
+notation ρ"["d"./"n"]" => subst_ρ ρ n d
+
 @[simp]
-def subst_sigma (σ : Var → Set α) (x : Var) (d : Set α) : Var → Set α :=
+def subst_σ (σ : Var → Set α) (x : Var) (d : Set α) : Var → Set α :=
   fun y => if y = x then d else σ y
 
+-- We need to define a shifting function in order to use the De Bruijn notation
 @[simp]
 def DeBruijnShift (ρ : ℕ → Set α ): ℕ → Set α :=
   fun n => ρ (n - 1)
 
+-- We implement the inductive defintion from 2.27 of our model interpretation of untyped lambda terms
 @[simp]
 def Interp (ρ : ℕ → Set α) (σ: Var → Set α) : Term Var → Set α
 | fvar x  => (σ x)
 | bvar n  => (ρ n)
 | app a b => (F (Interp ρ σ a) (Interp ρ σ b))
-| Term.abs e   =>  G (fun d => (Interp (subst_rho (DeBruijnShift ρ) 0 d) σ e) )
+| Term.abs e   =>  G (fun d => (Interp ((DeBruijnShift ρ)[d./0]) σ e) )
 
 variable {ρ : ℕ → Set α}
 variable {σ : Var → Set α}
@@ -41,74 +45,61 @@ variable {M N: Term Var}
 notation "〚"M"〛_{"ρ","σ"}" => Interp ρ σ M
 
 def K : Term Var := abs (abs $ bvar 1) -- λxy.x
-def I : Term Var := abs (bvar 0)
+def I : Term Var := abs (bvar 0)       -- λx. x
 
 -- We interp our I and K to see if our definition is well-defined according to our paper
 -- Example 3.1
-lemma interp_id :
-〚 I 〛_{ρ,σ} = {x | ∃ b, ∃ (β : α), x = (pair b β) ∧ b ∈ toSet β}
- := by
-  unfold I Interp G
+omit [DecidableEq Var] [HasFresh Var] in
+lemma interp_I :
+〚 I 〛_{ρ,σ} = {x | ∃ b, ∃ (β : α), x = (pair b β) ∧ b ∈ toSet β} := by
   ext x
   constructor
-  · intro h
-    obtain ⟨b, ⟨β, ⟨h₁, h₂⟩⟩⟩ := h
+  · rintro ⟨b, ⟨β, ⟨h₁, h₂⟩⟩⟩
     use b, β
-    constructor
-    · assumption
-    · dsimp [Interp] at h₂
-      assumption
-  · intro h
-    obtain ⟨b, ⟨β, ⟨h₁, h₂⟩⟩⟩ := h
+    simp at h₂
+    constructor <;> assumption
+  · rintro ⟨b, ⟨β, ⟨h₁, h₂⟩⟩⟩
     use b, β
-    constructor
-    · assumption
-    · dsimp [Interp]
-      assumption
+    constructor <;> assumption
 
+omit [DecidableEq Var] [HasFresh Var] in
 lemma interp_K:
-〚 K 〛_{ρ,σ} = {x | ∃ β γ c, x = (pair (pair c γ) β) ∧ c ∈ toSet β}
- := by
-  unfold K
-  unfold Interp
-  unfold G
+〚 K 〛_{ρ,σ} = {x | ∃ β γ c, x = (pair (pair c γ) β) ∧ c ∈ toSet β} := by
+  unfold K Interp G
   ext x
   simp
   constructor
-  · intro h
-    obtain ⟨b, β, h₁, h₂⟩ := h
-    obtain ⟨c, γ, heq, h₂⟩ := h₂
+  · rintro  ⟨b, β, h₁, ⟨c, γ, heq, h₂⟩⟩
     use β, γ, c
     constructor
     · rwa [heq] at h₁
-    · grind
-  · intro h
-    obtain ⟨β, γ, c, h⟩ := h
+    · grind only
+  · intro  ⟨β, γ, c, h⟩
     use ((pair c γ)), β
     constructor
     · grind
     · unfold G
       simp
-      grind
+      grind only
 
 ---------------------------------------------------------------------------------
 
 open GraphModel
 
 lemma env_comm {α : Type} (n : ℕ) (ρ : ℕ → Set α) (d es: Set α) :
-  subst_rho (DeBruijnShift (subst_rho ρ n d)) 0 es =
-  subst_rho (subst_rho (DeBruijnShift ρ) 0 es) (n + 1) d := by
+  subst_ρ (DeBruijnShift (subst_ρ ρ n d)) 0 es =
+  subst_ρ (subst_ρ (DeBruijnShift ρ) 0 es) (n + 1) d := by
     ext z _
     cases z with
     | zero => simp
     | succ z => simp
 
-
+omit [HasFresh Var] in
 lemma interp_open_rec (M : Term Var) (n : ℕ) (x : Var) (hx : x ∉ M.fv) (d : Set α) (ρ : ℕ → Set α) (σ : Var → Set α) :
-  Interp (subst_rho ρ n d) σ M = Interp ρ (subst_sigma σ x d) (openRec n (fvar x) M) := by
+  Interp (subst_ρ ρ n d) σ M = Interp ρ (subst_σ σ x d) (openRec n (fvar x) M) := by
   induction M generalizing n ρ with
   | fvar y =>
-    simp only [Interp, openRec, subst_sigma, right_eq_ite_iff]
+    simp only [Interp, openRec, subst_σ, right_eq_ite_iff]
     have : y ≠ x := by grind
     simp [this]
   | bvar m =>
@@ -153,7 +144,7 @@ lemma interp_rho_indep (M : Term Var) (ρ₁ ρ₂ : ℕ → Set α) (σ : Var �
     have ⟨f, f_fresh⟩ := fresh_exists exl_vars
     have h_f_notin_fvO : f ∉ O.fv := by grind only [= Finset.mem_union]
     have h_f_notin_L : f ∉ L := by grind only [= Finset.mem_union]
-    specialize ih f h_f_notin_L (DeBruijnShift ρ₁) (DeBruijnShift ρ₂) (subst_sigma σ f ds)
+    specialize ih f h_f_notin_L (DeBruijnShift ρ₁) (DeBruijnShift ρ₂) (subst_σ σ f ds)
     rw [interp_open_rec O 0 f h_f_notin_fvO ds (DeBruijnShift ρ₁) σ]
     rw [interp_open_rec O 0 f h_f_notin_fvO ds (DeBruijnShift ρ₂) σ]
     simp [open'] at ih
@@ -164,7 +155,7 @@ lemma interp_rho_indep (M : Term Var) (ρ₁ ρ₂ : ℕ → Set α) (σ : Var �
 
 -- 2.7 Substitution
 lemma DeBruijnSubst (M P : Term Var) (h : P.LC) (n : ℕ) (ρ : ℕ → Set α) (σ : Var → Set α) :
-  〚M〛_{subst_rho ρ n 〚P〛_{ρ,σ}, σ} = 〚openRec n P M〛_{ρ,σ} := by
+  〚M〛_{subst_ρ ρ n 〚P〛_{ρ,σ}, σ} = 〚openRec n P M〛_{ρ,σ} := by
   induction M generalizing n ρ with
   | bvar m =>
     simp [openRec, Interp]
@@ -184,16 +175,17 @@ lemma DeBruijnSubst (M P : Term Var) (h : P.LC) (n : ℕ) (ρ : ℕ → Set α) 
     rw [env_comm]
     let exl_vars := e.fv ∪ P.fv
     have ⟨f, f_fresh⟩ := fresh_exists exl_vars
-    have := interp_rho_indep P ρ (subst_rho (DeBruijnShift ρ) 0 ds) σ h
-    rw [this, ih (n + 1) (subst_rho (DeBruijnShift ρ) 0 ds)]
+    have := interp_rho_indep P ρ (subst_ρ (DeBruijnShift ρ) 0 ds) σ h
+    rw [this, ih (n + 1) (subst_ρ (DeBruijnShift ρ) 0 ds)]
 
 lemma G_cont (f : Set α → Set α → Set α) (h : ∀ S : Set α, continuous (f S)) :
 continuous fun S ↦ G (fun T ↦ f S T) := by
   sorry -- SORRY
 
+omit [DecidableEq Var] [HasFresh Var] in
 lemma DeBruijnSubst_continuous (P : Term Var) (i : ℕ)
 (ρ : ℕ → Set α) (σ : Var → Set α) :
-continuous fun d ↦ 〚P〛_{subst_rho (DeBruijnShift ρ) i d,σ} := by
+continuous fun d ↦ 〚P〛_{subst_ρ (DeBruijnShift ρ) i d,σ} := by
   induction P generalizing i ρ with
   | bvar n =>
     simp
@@ -216,7 +208,7 @@ continuous fun d ↦ 〚P〛_{subst_rho (DeBruijnShift ρ) i d,σ} := by
     unfold Interp
     apply G_cont
     intro a
-    specialize ih 0 (subst_rho (DeBruijnShift ρ) i a)
+    specialize ih 0 (subst_ρ (DeBruijnShift ρ) i a)
     exact ih
 
 ---------------------------------------------------------------------------------
@@ -227,9 +219,8 @@ lemma interp_ξ (xs : Finset Var)
 := by
   dsimp [Interp]
   congr 2
-  ext d a
-  let exl_vars := M.fv ∪ N.fv ∪ xs
-  have ⟨f, f_fresh⟩ := fresh_exists exl_vars
+  ext d _
+  have ⟨f, f_fresh⟩ := fresh_exists (M.fv ∪ N.fv ∪ xs)
 
   have hM : f ∉ M.fv := by grind
   have hN : f ∉ N.fv := by grind
@@ -237,18 +228,12 @@ lemma interp_ξ (xs : Finset Var)
 
   rw [interp_open_rec M 0 f hM d (DeBruijnShift ρ) σ]
   rw [interp_open_rec N 0 f hN d (DeBruijnShift ρ) σ]
-  specialize h f hxs (DeBruijnShift ρ) (subst_sigma σ f d)
+  specialize h f hxs
   simp [open'] at h
   rw [h]
 
 ---------------------------------------------------------------------------------
 
--- Prove Interp is a λ-theory
-
-open LT
-
-def InterpRel (M N : Term Var) : Prop :=
-  ∀ (ρ : ℕ → Set α) (σ : Var → Set α), 〚M〛_{ρ,σ} = 〚N〛_{ρ,σ}
 
 -- Prove beta-step entails model interpretation equality
 lemma beta_step_imp_interp_eq (ρ : ℕ → Set α) (σ : Var → Set α)
@@ -261,14 +246,13 @@ lemma beta_step_imp_interp_eq (ρ : ℕ → Set α) (σ : Var → Set α)
       expose_names
       simp only [Interp]
       rw [F_G_eq_id]
-      · change 〚M〛_{subst_rho (DeBruijnShift ρ) 0 〚b〛_{ρ,σ}, σ} = 〚M⟦0 ↝ b⟧〛_{ρ,σ}
-        have hb_shift : 〚b〛_{ρ, σ} = 〚b〛_{DeBruijnShift ρ, σ} := interp_rho_indep b _ _ _ hb
+      · have hb_shift : 〚b〛_{ρ, σ} = 〚b〛_{DeBruijnShift ρ, σ} := interp_rho_indep b _ _ _ hb
         rw [hb_shift]
 
-        have h_reduced_LC : (M⟦0 ↝ b⟧).LC := by exact LC_of_absLC_and_LC_term M b hM hb
+        have h_reduced_LC : (M ^ b).LC := beta_lc hM hb
 
-        have rhs_shift : 〚M⟦0 ↝ b⟧〛_{ρ, σ} = 〚M⟦0 ↝ b⟧〛_{DeBruijnShift ρ, σ} :=
-          interp_rho_indep (M⟦0 ↝ b⟧) _ _ _ h_reduced_LC
+        have rhs_shift : 〚M ^ b〛_{ρ, σ} = 〚M ^ b〛_{DeBruijnShift ρ, σ} :=
+          interp_rho_indep (M ^ b) _ _ _ h_reduced_LC
 
         rw [rhs_shift]
 
@@ -276,18 +260,16 @@ lemma beta_step_imp_interp_eq (ρ : ℕ → Set α) (σ : Var → Set α)
       · apply DeBruijnSubst_continuous
     | _ => contradiction
   · expose_names
-    simp
-    rw [a_ih]
+    simp only [Interp, a_ih]
   · expose_names
-    simp
-    rw [a_ih]
+    simp only [Interp, a_ih]
   · expose_names
     simp at h
     apply interp_ξ xs
     · intro x hx ρ σ
       apply a_ih x hx ρ σ
 
--- Prove multi-beta-step entails model interpretation equality
+-- Prove ↠βᶠ entails model interpretation equality
 lemma multi_beta_imp_interp_eq (ρ : ℕ → Set α) (σ : Var → Set α) (A B : Term Var):
 (A ↠βᶠ B) -> 〚 A 〛_{ρ,σ} = 〚 B 〛_{ρ,σ}
  := by
@@ -298,7 +280,7 @@ lemma multi_beta_imp_interp_eq (ρ : ℕ → Set α) (σ : Var → Set α) (A B 
    rw [a_ih]
    apply (beta_step_imp_interp_eq ρ σ h_1)
 
--- Prove beta-equality entails model interpretation equality
+-- Prove β-equivalence entails model interpretation equality
 lemma beta_eq_imp_interp_eq (ρ : ℕ → Set α) (σ : Var → Set α) (A B : Term Var):
 (A ≡β B) -> 〚 A 〛_{ρ,σ} = 〚 B 〛_{ρ,σ}
   := by
@@ -307,6 +289,14 @@ lemma beta_eq_imp_interp_eq (ρ : ℕ → Set α) (σ : Var → Set α) (A B : T
   rw [multi_beta_imp_interp_eq ρ σ _ _ hmB]
   exact multi_beta_imp_interp_eq ρ σ _ _ hmA
 
+--------------------------------------------------------------------------------
+open LT
+
+-- We define the theory of this model to be equations generated by equality in the model
+def InterpRel (M N : Term Var) : Prop :=
+  ∀ (ρ : ℕ → Set α) (σ : Var → Set α), 〚M〛_{ρ,σ} = 〚N〛_{ρ,σ}
+
+-- Finally, prove that the set of equations from Interp is a λ-theory
 instance : LambdaTheory (fun (M N : Term Var) => @InterpRel Var α _ M N) where
   beta M N h ρ σ := by
     apply beta_eq_imp_interp_eq
@@ -320,6 +310,3 @@ instance : LambdaTheory (fun (M N : Term Var) => @InterpRel Var α _ M N) where
   refl M ρ σ := by rfl
   trans M N Q hMN hNQ ρ σ := (hMN ρ σ).trans (hNQ ρ σ)
   sym M N h ρ σ := (h ρ σ).symm
-
---------------------------------------------------------------------------------
--- Prove beta-equvialence entails model interpretation equality
