Project/AndrejBauer/CombinatoryAlgebra.lean
@@ -1,7 +1,7 @@
 import Mathlib.Tactic.NthRewrite
 import Mathlib.Data.Part
-import src.AndrejBauer.Basic
-import src.AndrejBauer.PartialCombinatoryAlgebra
+import Project.AndrejBauer.Basic
+import Project.AndrejBauer.PartialCombinatoryAlgebra
 
 /-- A (total) combinatory structure on a set `A`. -/
 class CA (A : Type*) extends HasDot A where
